lib/ext.fst
@@ -1,9 +1,8 @@
 module Extensionality
+type arr (a:Type) (b:Type) = a -> Tot b
 
-type arr (a:Type) (b:(a->Type)) = x:a -> Tot (b x)
+opaque logic type Eq : #a:Type -> #b:Type -> arr a b -> arr a b -> Type =
+           fun (a:Type) (b:Type) (f:arr a b) (g:arr a b) -> (forall x. f x = g x)
 
-opaque type Eq : #a:Type -> #b:(a -> Type) -> arr a b -> arr a b -> Type = 
-           fun (a:Type) (b:(a->Type)) (f:arr a b) (g:arr a b) -> (forall x. f x = g x)
-
-assume Extensionality : forall (a:Type) (b:(a->Type)) (f: arr a b) (g: arr a b).
+assume Extensionality : forall (a:Type) (b:Type) (f: arr a b) (g: arr a b).
                         {:pattern Eq #a #b f g} Eq #a #b f g <==> f=g
